Set bullets to strict mode

syntax.sig
@@ -1,9 +1,10 @@
 tm : Type
 nat : Type
+grade : Type
 
-tAbs : tm -> (tm -> tm) -> tm
-tApp : tm -> tm -> tm
-tPi : tm -> (tm -> tm) -> tm
+tAbs : grade -> tm -> (tm -> tm) -> tm
+tApp : tm -> grade -> tm -> tm
+tPi : grade -> tm -> (tm -> tm) -> tm
 tFalse : tm
 tUniv : nat -> tm
 tOn : tm
